ver2/optimizations/eval.v
@@ -1,0 +1,171 @@
+Require Import bbv.Word.
+Require Import Nat. 
+Require Import Coq.NArith.NArith.
+
+Require Import Coq.Logic.FunctionalExtensionality.
+
+Require Import FORVES.constants.
+Import Constants.
+
+Require Import FORVES.symbolic_state.
+Import SymbolicState.
+
+Require Import FORVES.symbolic_state_eval.
+Import SymbolicStateEval.
+
+Require Import FORVES.symbolic_state_cmp.
+Import SymbolicStateCmp.
+
+Require Import FORVES.valid_symbolic_state.
+Import ValidSymbolicState.
+
+Require Import FORVES.execution_state.
+Import ExecutionState.
+
+Require Import FORVES.stack_operation_instructions.
+Import StackOpInstrs.
+
+Require Import FORVES.program.
+Import Program.
+
+Require Import FORVES.symbolic_state_cmp_impl.
+Import SymbolicStateCmpImpl.
+
+Require Import FORVES.symbolic_state_eval_facts.
+Import SymbolicStateEvalFacts.
+
+Require Import FORVES.valid_symbolic_state.
+Import ValidSymbolicState.
+
+Require Import FORVES.misc.
+Import Misc.
+
+Require Import FORVES.eval_common.
+Import EvalCommon.
+
+Require Import FORVES.concrete_interpreter.
+Import ConcreteInterpreter.
+
+Require Import FORVES.optimizations_def.
+Import Optimizations_Def.
+
+Require Import FORVES.optimizations_common.
+Import Optimizations_Common.
+
+Require Import List.
+Import ListNotations.
+
+
+Module Opt_eval.
+
+
+(* EVAL *)
+Definition optimize_eval_sbinding : opt_smap_value_type := 
+fun (val: smap_value) =>
+fun (fcmp: sstack_val_cmp_t) =>
+fun (sb: sbindings) =>
+fun (maxid: nat) =>
+fun (instk_height: nat) =>
+fun (ops: stack_op_instr_map) => 
+match val with
+| SymOp op args => 
+  match follow_to_val_args args maxid sb with
+  | Some vargs => 
+    match ops op with
+    | OpImp nargs f Hcomm Hctx_indep => 
+      match Hctx_indep with
+      | Some _ => if (List.length args =? nargs) then
+                    (SymBasicVal (Val (f empty_context vargs)), true)
+                  else 
+                    (val, false)
+      | None => (val, false)
+      end
+    end
+  | None => (val, false)
+  end
+| _ => (val, false)
+end.
+
+
+
+
+
+
+Lemma optimize_eval_sbinding_smapv_valid:
+opt_smapv_valid_snd optimize_eval_sbinding.
+Proof.
+unfold opt_smapv_valid_snd.
+intros instk_height n ops fcmp sb val val' flag.
+intros Hvalid_smapv_val Hvalid_sb Hoptm_sbinding.
+unfold optimize_eval_sbinding in Hoptm_sbinding.
+destruct (val) as [basicv|pushtagv|label args|offset smem|key sstrg|
+  offset size smem] eqn: eq_val; try (
+    injection Hoptm_sbinding as eq_val' _;
+    rewrite <- eq_val';
+    assumption).
+(* SymOp label args *)
+destruct (follow_to_val_args args n sb) as [vargs|] eqn: eq_follow; 
+  try inject_rw Hoptm_sbinding eq_val'.
+destruct (ops label) as [nargs f Hcomm Hctx_indep] eqn: eq_ops_label; 
+  try inject_rw Hoptm_sbinding eq_val'.
+destruct (Hctx_indep) as [H|]; try inject_rw Hoptm_sbinding eq_val'.
+destruct (length args =? nargs); try inject_rw Hoptm_sbinding eq_val'.
+injection Hoptm_sbinding as eq_val' _.
+rewrite <- eq_val'.
+simpl. intuition.
+Qed.
+
+
+Lemma optimize_eval_sbinding_snd:
+opt_sbinding_snd optimize_eval_sbinding.
+Proof.
+unfold opt_sbinding_snd.
+intros val val' fcmp sb maxidx instk_height idx flag Hsafe_sstack_val_cmp
+  Hvalid Hoptm_sbinding.
+split.
+- (* valid_sbindings *)
+  apply valid_bindings_snd_opt with (val:=val)(opt:=optimize_eval_sbinding)
+    (fcmp:=fcmp)(flag:=flag); try assumption.
+  apply optimize_eval_sbinding_smapv_valid. 
+    
+- (* evaluation is preserved *) 
+  intros stk mem strg ctx v Hlen Heval_orig.
+  (*assert (Hlen2 := Hlen).
+  rewrite -> Hlen in Hlen2.
+  rewrite <- Hlen in Hlen2 at 2.*)
+  unfold optimize_eval_sbinding in Hoptm_sbinding.
+  (*pose proof (Hvalid_maxidx instk_height maxidx idx val sb evm_stack_opm
+      Hvalid) as eq_maxidx_idx.*)
+  destruct val as [vv|vv|label args|offset smem|key sstrg|offset seze smem]
+    eqn: eq_val; try inject_rw Hoptm_sbinding eq_val'.
+  (* SymOp label args *)
+  destruct (follow_to_val_args args idx sb) as [vargs|] eqn: eq_follow; 
+  try inject_rw Hoptm_sbinding eq_val'.
+  destruct (evm_stack_opm label) as [nargs f Hcomm Hctx_indep] 
+    eqn: eq_ops_label; try inject_rw Hoptm_sbinding eq_val'.
+  destruct (Hctx_indep) as [H|] eqn: eq_Hctx; 
+    try inject_rw Hoptm_sbinding eq_val'.
+  destruct (length args =? nargs) eqn: eq_len; 
+    try inject_rw Hoptm_sbinding eq_val'.
+  injection Hoptm_sbinding as eq_val' _.
+  rewrite <- eq_val'.
+  unfold eval_sstack_val. simpl.
+  rewrite -> PeanoNat.Nat.eqb_refl.
+  unfold eval_sstack_val in Heval_orig. simpl in Heval_orig.
+  rewrite -> PeanoNat.Nat.eqb_refl in Heval_orig.
+  rewrite -> eq_ops_label in Heval_orig.
+  rewrite -> eq_len in Heval_orig.
+  destruct (map_option
+                 (fun sv' : sstack_val =>
+                  eval_sstack_val' maxidx sv' stk mem strg ctx idx sb
+                    evm_stack_opm) args) as [vargs'|] eqn: eq_mapo;
+    try discriminate.
+  pose proof (follow_to_val_args_eval_eq args idx sb vargs maxidx stk mem 
+    strg ctx vargs' eq_follow eq_mapo) as eq_vargs'.
+  rewrite <- eq_vargs' in Heval_orig.
+  rewrite -> H with (ctx2:=ctx).
+  assumption.
+Qed.
+
+
+End Opt_eval.
